Final Version
Proved everything, including Lemmas + added annotated versions

MatrixDiagonals.dfy
@@ -90,6 +90,134 @@ function MatrixDiagSum(m: array2<int>, N: nat, d: nat): int
 	SumOnD(m, N, d, 0, 0, 0)
 } 
 
+function SumOnD(m: array2<int>, N: nat, d: nat, i: nat, j: nat, sum: int): int
+	requires m != null && d < N == m.Length0 == m.Length1 && i <= N && j <= N
+	decreases N-i, N-j
+	reads m
+{
+	if i == N then sum else
+	if j == N then SumOnD(m, N, d, i+1, 0, sum) else
+	if Abs(i-j) == d then SumOnD(m, N, d, i, j+1, sum+m[i,j]) else
+	SumOnD(m, N, d, i, j+1, sum)
+}
+
+function Abs(n: int): nat { if n>=0 then n else -n }
+
+method MatrixDiagonal(m: array2<int>, N:nat, d:nat) returns (s:int)
+	requires m!=null && d<N == m.Length0 == m.Length1
+	ensures s==MatrixDiagSum(m,N,d)
+	{
+		s:=0;
+		var i: int :=0;
+		assert MatrixDiagSum(m,N,d) == SumOnD(m,N,d,i,0,s);
+
+		while i!=N
+			invariant i<=N
+			invariant MatrixDiagSum(m,N,d) == SumOnD(m,N,d,i,0,s)
+			decreases N-i
+		{
+
+				if(i-d>=0) //i-d>=0
+				{	
+					//covering the skippable gap between m[i,0] to m[i,i-d]
+					assert SumOnD(m,N,d,i,0,s)==SumOnD(m,N,d,i,i-d,s) by {LooperRow(m,N,d,i,0,i-d,s);}
+					//adding the element at m[i,i-d]
+					assert SumOnD(m,N,d,i,i-d,s)==SumOnD(m,N,d,i,i-d+1,s+m[i,i-d]) by {L2(m,N,d,i,i-d,s);} 
+					s:=s+m[i,i-d];
+					if(i+d<N) //i-d>=0 and i+d<N
+					{
+						if(d==0) //meaning i-d==i+d, i-d>=0 and i+d<N
+						{
+							//covering the skippable gap between m[i,i-d+1] to m[i,N]
+							assert d==0;
+							assert SumOnD(m,N,d,i,i-d+1,s)==SumOnD(m,N,d,i,N,s) by {LooperRow(m,N,d,i,i-d+1,N,s);}
+						}
+						else //i-d>=0 and i+d<N and d!=0
+						{
+							//covering the skippable gap between m[i,i-d+1] to m[i,i-d+1,i+d]
+							assert d!=0;
+							assert SumOnD(m,N,d,i,i-d+1,s)==SumOnD(m,N,d,i,i+d,s) by {LooperRow(m,N,d,i,i-d+1,i+d,s);}
+
+							//adding the element at m[i,i+d]
+							assert SumOnD(m,N,d,i,i+d,s)==SumOnD(m,N,d,i,i+d+1,s+m[i,i+d]) by {L2(m,N,d,i,i+d,s);} 
+
+							s:=s+m[i,i+d];
+
+							//covering all the skippable gap between m[i,i+d+1] to m[i,N]
+							assert SumOnD(m,N,d,i,i+d+1,s)==SumOnD(m,N,d,i,N,s) by {LooperRow(m,N,d,i,i+d+1,N,s);}					
+						}
+					}
+					else //i-d>=0 and !(i+d<N)
+					{
+						//covering the skippable gap between m[i,i-d+1] to m[i,N]
+						assert SumOnD(m,N,d,i,i-d+1,s)==SumOnD(m,N,d,i,N,s) by {LooperRow(m,N,d,i,i-d+1,N,s);}
+					}
+			}
+			else // !(i-d>=0)
+			{
+				if(i+d<N){ // !(i-d>=0) and i+d<N
+					//covering the skippable gap between m[i,0] to m[i,i+d]
+					assert SumOnD(m,N,d,i,0,s)==SumOnD(m,N,d,i,i+d,s) by {LooperRow(m,N,d,i,0,i+d,s);}
+
+					//adding the element at m[i,i+d] to s
+					assert SumOnD(m,N,d,i,i+d,s)==SumOnD(m,N,d,i,i+d+1,s+m[i,i+d]) by {L2(m,N,d,i,i+d,s);} 
+
+					s:=s+m[i,i+d];
+					
+					//covering the skipppable gap between m[i,i+d+1] to m[i,N]
+					assert SumOnD(m,N,d,i,i+d+1,s)==SumOnD(m,N,d,i,N,s) by {LooperRow(m,N,d,i,i+d+1,N,s);}
+						
+				}
+				else // !(i-d>=0) and !(i+d<N)
+				{
+					//covering the skippable gap between m[i,0] to m[i,N]
+					assert SumOnD(m,N,d,i,0,s)==SumOnD(m,N,d,i,N,s) by {LooperRow(m,N,d,i,0,N,s);}
+					
+				}
+			}
+				
+			assert i+1<=N &&MatrixDiagSum(m,N,d) == SumOnD(m,N,d,i+1,0,s);
+			i:=i+1;
+			assert i<=N && MatrixDiagSum(m,N,d) == SumOnD(m,N,d,i,0,s);
+		}
+
+		assert i==N && i<=N && MatrixDiagSum(m,N,d) == SumOnD(m,N,d,i,0,s);
+		// ==> {SumOnD(m,N,d,i,0,s) == SumOnD(m, N, d, N, 0, s) (because i==N) == s (by definition) }
+		assert s == MatrixDiagSum(m,N,d);
+		
+	}
+
+// a and b refer to the start and end indexes of j meaning from m[i,a] to m[i,b] 
+//all elements m[i,k] ==> Abs(i-k)!=d
+lemma LooperRow(m:array2<int>, N:nat, d:nat, i:nat, a:nat, b:nat, s:int)
+requires m != null && d < N == m.Length0 == m.Length1 && i < N 
+requires forall x:nat :: a <= x < b ==> (if (i-x)>=0 then (i-x) else -(i-x)) != d
+requires  0<=a<=b<=N
+ensures SumOnD(m,N,d,i,a,s)== SumOnD(m,N,d,i,b,s)
+{	
+	assert forall x:nat :: a <= x < b ==> (if (i-x)>=0 then (i-x) else -(i-x)) != d;
+	var k:=a;
+	while k!=b
+		invariant a<=k<=b && SumOnD(m,N,d,i,a,s)==SumOnD(m,N,d,i,k,s)
+	{	
+		assert a<=k+1<=b && SumOnD(m,N,d,i,a,s)==SumOnD(m,N,d,i,k+1,s) by 
+		{
+			calc{
+					SumOnD(m,N,d,i,a,s);
+					== 
+					SumOnD(m,N,d,i,k,s);
+					== 
+					{
+						L1(m,N,d,i,k,s);
+					}
+					SumOnD(m,N,d,i,k+1,s);
+				}	
+		}
+		k:=k+1;
+	}
+	assert k==b && a<=k<=b && SumOnD(m,N,d,i,a,s)==SumOnD(m,N,d,i,k,s);
+	assert SumOnD(m,N,d,i,a,s)== SumOnD(m,N,d,i,b,s);
+}
 
 lemma L1(m: array2<int>, N: nat, d: nat, i: nat, j: nat, s: int)
 	// an irrelevant element a[i,j] (with "Abs(i-j) != d") can be skipped...
@@ -107,7 +235,6 @@ lemma L1(m: array2<int>, N: nat, d: nat, i: nat, j: nat, s: int)
 	}
 }
 
-
 lemma L2(m:array2<int>, N:nat, d:nat, i:nat, j:nat, s:int)
 	requires m!=null && d<N==m.Length0 == m.Length1
 	requires i<N
@@ -123,278 +250,206 @@ lemma L2(m:array2<int>, N:nat, d:nat, i:nat, j:nat, s:int)
 		}
 	}
 
-/**lemma ShwoopDeLoop(m: array2<int>, N:nat, d:nat, i:nat, j:nat, s:int)
-	requires m != null && d < N == m.Length0 == m.Length1 && i <= N && j <= N
-	ensures MatrixDiagSum(m,N,d) == SumOnD(m,N,d,i,j,s)
-	{
-		assert (MatrixDiagSum(m,N,d) == SumOnD(m,N,d,i,j,s)) ==> (MatrixDiagSum(m,N,d) == s + SumOnD(m,N,d,i,j,0) ) ; 
-	}
-	*/
-	/**
-lemma Looper(m: array2<int>, N:nat, d:nat, i:nat, j:nat, s:int)
-	requires m!=null &&d<N==m.Length0 == m.Length1
-	requires i<=N
-	requires j<N
-	ensures MatrixDiagSum(m,N,d) == SumOnD(m,N,d,i,j,s)
-	//I want to say that SumOnD(m,N,d,i,j,s) is equal to the s we would receive if we summed up all the correct values up to m[i,j]
-	//plus SumOnD(m,N,d,i,j,0)
-	{
-	var s':nat;
-	s':=0;
-		//for all k,l:nat | k>=0 && l>=0 && k<=i && k<j ensures SumOnD(m,n,d,i,j,s) == MatrixDiagSum(m,N,d)
-		
-		//here i really want to go over all the elements, and say that 
-		forall k,l:nat | k>=i && l>=j && k<N && l<N ensures MatrixDiagSum(m,N,d) == SumOnD(m,N,d,i,0,s')
-		{
-			if(Abs(k-l)==d){
-				assert Abs(k-l)==d;
-				L2(m,N,d,k,l,s);
-				assert SumOnD(m,N,d,k,l,s)== SumOnD(m,N,d,k,l+1,s+m[k,l]);
-			}
-			else{
-				assert Abs(k-l)!=d;
-				L1(m,N,d,k,l,s);
-				assert SumOnD(m,N,d,k,l,s) == SumOnD(m,N,d,k,l+1,s);
-			}
-		} 
-	}*/
 
+/** Annotated Versions (Inluding asserts) */
 
+/**
 
-function SumOnD(m: array2<int>, N: nat, d: nat, i: nat, j: nat, sum: int): int
-	requires m != null && d < N == m.Length0 == m.Length1 && i <= N && j <= N
-	decreases N-i, N-j
-	reads m
-{
-	if i == N then sum else
-	if j == N then SumOnD(m, N, d, i+1, 0, sum) else
-	if Abs(i-j) == d then SumOnD(m, N, d, i, j+1, sum+m[i,j]) else
-	SumOnD(m, N, d, i, j+1, sum)
-}
-
-function Abs(n: int): nat { if n>=0 then n else -n }
-
-method max(a: int, b: int) returns (s:int)
-{
-	//s:=0;
-	if a > b{	
-		s:=a;
-	} 
-	else{
-		s:=b;
-   }
-}
-
-method MatrixDiagonal(m: array2<int>, N:nat, d:nat) returns (s:int)
+method MatrixDiagonal'(m: array2<int>, N:nat, d:nat) returns (s:int)
 	requires m!=null && d<N == m.Length0 == m.Length1
 	ensures s==MatrixDiagSum(m,N,d)
 	{
-	
-	s:=0;
-	//ghost var s':=s;
-	var i: int :=0;
-	assert m!=null && d<N == m.Length0 == m.Length1;
-	assert MatrixDiagSum(m,N,d) == SumOnD(m,N,d,i,0,s);
-	assert s == MatrixDiagSum(m,N,d) - SumOnD(m,N,d,i,0,0);
+		s:=0;
+		var i: int :=0;
+		assert MatrixDiagSum(m,N,d) == SumOnD(m,N,d,i,0,s);
 
-	while i!=N
-		invariant i<=N
-		//what do i want to say?? i want to say that the sum i have accumulated so far, s,
-		//plus the rest of the valid elements in the array SumOnD(m,N,d,i,j,s) will be equal to the end result MatrixDiagSum(m,N,d)
-		//invariant MatrixDiagSum(m,N,d) == SumOnD(m,N,d,i,0,s)
-		//invariant s == MatrixDiagSum(m,N,d) - SumOnD(m,N,d,i,0,0)
-		decreases N-i
+		while i!=N
+			invariant i<=N
+			invariant MatrixDiagSum(m,N,d) == SumOnD(m,N,d,i,0,s)
+			decreases N-i
 		{
-			assert i<=N;
-			assert i<N;
-			//assert MatrixDiagSum(m,N,d) == SumOnD(m,N,d,i,0,s) by {Looper(m,N,d,i,0,s);}
-			//s':=s;
-
-			if(i-d-1>=0){
-				forall j:int | 0<=j<i-d  && i>d ensures SumOnD(m,N,d,i,j,s)==SumOnD(m,N,d,i,i-d-1,s) {L1(m,N,d,i,j,s);}
-				assert SumOnD(m,N,d,i,0,s)==SumOnD(m,N,d,i,i-d-1,s); 
+				assert i!=N && i<=N;
+				// ==>
+				assert i<N;
+				
+				if(i-d>=0) //i-d>=0
+				{	
+					//covering the skippable gap between m[i,0] to m[i,i-d]
+					assert i-d>=0;
+					assert SumOnD(m,N,d,i,0,s)==SumOnD(m,N,d,i,i-d,s) by 
+					{
+						assert m != null && d < N == m.Length0 == m.Length1 && i < N;
+						assert forall x:nat :: 0 <= x < i-d ==> Abs(i-x)!= d;
+						assert  0<=0<=i-d<=N;
+						LooperRow(m,N,d,i,0,i-d,s);
+					}
+					//adding the element at m[i,i-d]
+					assert SumOnD(m,N,d,i,i-d,s)==SumOnD(m,N,d,i,i-d+1,s+m[i,i-d]) by 
+					{
+						assert m!=null && d<N==m.Length0 == m.Length1 && i<N && i-d<N;
+						assert Abs(i-(i-d))==d;
+						L2(m,N,d,i,i-d,s);
+					} 
+					s:=s+m[i,i-d];
+					if(i+d<N) //i-d>=0 and i+d<N
+					{
+						assert i+d<N;
+						if(d==0) //meaning i-d==i+d, i-d>=0 and i+d<N
+						{
+							//covering the skippable gap between m[i,i-d+1] to m[i,N]
+							assert d==0;
+							assert SumOnD(m,N,d,i,i-d+1,s)==SumOnD(m,N,d,i,N,s) by
+							{	
+								assert m != null && d < N == m.Length0 == m.Length1 && i < N  && i-d+1<=N && N<=N;
+								assert 0<=i-d+1<=N<=N;
+								assert forall x :: i-d+1 <= x < N ==> Abs(i-x)!=d;
+								LooperRow(m,N,d,i,i-d+1,N,s);
+							}
+						}
+						else //i-d>=0 and i+d<N and d!=0
+						{
+							//covering the skippable gap between m[i,i-d+1] to m[i,i-d+1,i+d]
+							assert d!=0;
+							assert SumOnD(m,N,d,i,i-d+1,s)==SumOnD(m,N,d,i,i+d,s) by 
+							{	
+								assert m != null && d < N == m.Length0 == m.Length1 && i < N  && i-d+1<=N && i+d<=N;
+								assert 0<=i-d+1<=i+d<=N;
+								assert forall x :: i-d+1 <= x < i+d ==> Abs(i-x)!=d; 
+								LooperRow(m,N,d,i,i-d+1,i+d,s);
+							}
+							//adding the element at m[i,i+d]
+							assert SumOnD(m,N,d,i,i+d,s)==SumOnD(m,N,d,i,i+d+1,s+m[i,i+d]) by 
+							{
+								assert m!=null && d<N==m.Length0 == m.Length1 && i<N && i+d<N;
+								assert Abs(i-(i+d))==d;
+								L2(m,N,d,i,i+d,s);
+							} 
+							s:=s+m[i,i+d];
+							//covering all the skippable gap between m[i,i+d+1] to m[i,N]
+							assert SumOnD(m,N,d,i,i+d+1,s)==SumOnD(m,N,d,i,N,s) by 
+							{
+								assert m != null && d < N == m.Length0 == m.Length1 && i < N  && i+d+1<=N && N<=N;
+								assert 0<=i+d+1<=N<=N;
+								assert forall x :: i+d+1 <= x < N ==> Abs(i-x)!=d;
+								LooperRow(m,N,d,i,i+d+1,N,s);
+							}					
+						}
+					}
+					else //i-d>=0 and !(i+d<N)
+					{
+						//covering the skippable gap between m[i,i-d+1] to m[i,N]
+						assert SumOnD(m,N,d,i,i-d+1,s)==SumOnD(m,N,d,i,N,s) by 
+						{
+							assert m != null && d < N == m.Length0 == m.Length1 && i < N  && i-d+1<=N && N<=N;
+							assert 0<=i-d+1<=N<=N;
+							assert forall x :: i-d+1 <= x < N ==> Abs(i-x)!=d;
+							LooperRow(m,N,d,i,i-d+1,N,s);
+						}
+					}
 			}
+			else // !(i-d>=0)
+			{
+				if(i+d<N){ // !(i-d>=0) and i+d<N
+					//covering the skippable gap between m[i,0] to m[i,i+d]
+					assert SumOnD(m,N,d,i,0,s)==SumOnD(m,N,d,i,i+d,s) by 
+					{
+						assert m != null && d < N == m.Length0 == m.Length1 && i < N  && 0<=N && i+d<=N;
+						assert 0<=0<=i+d<=N;
+						assert forall x :: 0 <= x < i+d ==> Abs(i-x)!=d;
+						LooperRow(m,N,d,i,0,i+d,s);
+					}
 
-			ghost var maxValidJ:=max(0,i-d-1);
-			forall j:int | 0<=j<i-d  && i>d ensures SumOnD(m,N,d,i,j,s)==SumOnD(m,N,d,i,j+1,s) {
-				L1(m,N,d,i,j,s);
-			}
-			assert SumOnD(m,N,d,i,0,s)==SumOnD(m,N,d,i,maxValidJ,s); 
+					//adding the element at m[i,i+d] to s
+					assert SumOnD(m,N,d,i,i+d,s)==SumOnD(m,N,d,i,i+d+1,s+m[i,i+d]) by 
+					{
+						assert m!=null && d<N==m.Length0 == m.Length1 && i<N && i+d<N;
+						assert Abs(i-(i+d))==d;
+						L2(m,N,d,i,i+d,s);
+					} 
 
-			//forall k:nat | 0<=k<d-i && i-k>=0 && i-k>d ensures SumOnD(m,N,d,i,0,s)==SumOnD(m,N,d,i,k,s) {L1(m,N,d,i,k,s);}
-
-			if(i-d>=0){
-				s:=s+m[i,i-d];
-
-				if(i+d<N){
 					s:=s+m[i,i+d];
+					
+					//covering the skipppable gap between m[i,i+d+1] to m[i,N]
+					assert SumOnD(m,N,d,i,i+d+1,s)==SumOnD(m,N,d,i,N,s) by 
+					{
+						assert m != null && d < N == m.Length0 == m.Length1 && i < N  && i+d+1<=N && N<=N;
+						assert 0<=i+d+1<=N<=N;
+						assert forall x :: i+d+1 <= x < N ==> Abs(i-x)!=d;
+						LooperRow(m,N,d,i,i+d+1,N,s);
+					}
+						
 				}
-				else{
+				else // !(i-d>=0) and !(i+d<N)
+				{
+					//covering the skippable gap between m[i,0] to m[i,N]
+					assert SumOnD(m,N,d,i,0,s)==SumOnD(m,N,d,i,N,s) by 
+					{
+						assert m != null && d < N == m.Length0 == m.Length1 && i < N  && 0<=N && N<=N;
+						assert 0<=0<=N<=N;
+						assert forall x :: 0 <= x < N ==> Abs(i-x)!=d;
+						LooperRow(m,N,d,i,0,N,s);
+					}
 					
 				}
 			}
-			else{
-				//Took nothing so far..
-				if(i+d<N){
-					s:=s+m[i,i+d];
-				}
-				else{
-				}
-			}
-
-			forall k:nat | 0<=k<d+i && i-k<N && i-k>=0 && i-k<d ensures SumOnD(m,N,d,i,0,s)==SumOnD(m,N,d,i,k,s) {L1(m,N,d,i,k,s);}
-
+				
+			assert i+1<=N &&MatrixDiagSum(m,N,d) == SumOnD(m,N,d,i+1,0,s);
 			i:=i+1;
-
+			assert i<=N && MatrixDiagSum(m,N,d) == SumOnD(m,N,d,i,0,s);
 		}
 
+		assert i==N && i<=N && MatrixDiagSum(m,N,d) == SumOnD(m,N,d,i,0,s);
+		// ==> {SumOnD(m,N,d,i,0,s) == SumOnD(m, N, d, N, 0, s) (because i==N) == s (by definition) }
+		assert s == MatrixDiagSum(m,N,d);
 		
-		assert i==N;
-		//assert MatrixDiagSum(m,N,d) == SumOnD(m,N,d,i,N,s); //by { LoopingLemma(m,N,d,i,s); }
-		assert s == MatrixDiagSum(m,N,d);
-
 	}
+	
 
-	method MatrixDiagonal2(m: array2<int>, N:nat, d:nat) returns (s:int)
-	requires m!=null && d<N == m.Length0 == m.Length1
-	ensures s==MatrixDiagSum(m,N,d)
-	{
-	s:=0;
-	var i: int :=0;
-	assert m!=null && d<N == m.Length0 == m.Length1;
-	assert MatrixDiagSum(m,N,d) == SumOnD(m,N,d,i,0,s);
 
-	assert MatrixDiagSum(m,N,d) == SumOnD(m,N,d,i,0,s);
-	while i!=N
-		invariant i<=N
-		invariant MatrixDiagSum(m,N,d) == SumOnD(m,N,d,i,0,s)
-		decreases N-i
+// a and b refer to the start and end indexes of j meaning from m[i,a] to m[i,b] 
+//every element m[i,k] ==> Abs(i-k)!=d
+lemma LooperRow'(m:array2<int>, N:nat, d:nat, i:nat, a:nat, b:nat, s:int)
+requires m != null && d < N == m.Length0 == m.Length1 && i < N 
+requires forall x:nat :: a <= x < b ==> (if (i-x)>=0 then (i-x) else -(i-x)) != d
+requires  0<=a<=b<=N
+ensures SumOnD(m,N,d,i,a,s)== SumOnD(m,N,d,i,b,s)
+{	
+	assert m != null && d < N == m.Length0 == m.Length1 && i < N;
+	assert forall x:nat :: a <= x < b ==> (if (i-x)>=0 then (i-x) else -(i-x)) != d;
+	assert 0<=a<=b<=N;
+
+	var k:=a;
+
+	while k!=b
+		invariant a<=k<=b && SumOnD(m,N,d,i,a,s)==SumOnD(m,N,d,i,k,s)
+	{	
+		assert a<=k+1<=b && SumOnD(m,N,d,i,a,s)==SumOnD(m,N,d,i,k+1,s) by 
 		{
-			assert MatrixDiagSum(m,N,d) == SumOnD(m,N,d,i,0,s);
-			assert i<N;
-			if(i+d<N){
-				//	forall k:nat ensures 0<=k && k<=i+d { L1(m,N,d,i,i+d,s);}
-				assert MatrixDiagSum(m,N,d) == SumOnD(m,N,d,i,0,s);
-				s:=s+m[i,i+d];
-				assert MatrixDiagSum(m,N,d) == SumOnD(m,N,d,i,0,s-m[i,i+d]);
-				if(i-d>=0){
-					assert MatrixDiagSum(m,N,d) == SumOnD(m,N,d,i,0,s-m[i,i+d]);
-					s:=s+m[i,i-d];
-					assert MatrixDiagSum(m,N,d) == SumOnD(m,N,d,i,0,s-m[i,i+d]-m[i,i-d]);
-				}
-				else{
-					assert MatrixDiagSum(m,N,d) == SumOnD(m,N,d,i,0,s-m[i,i+d]);
-				}
-			}
-			else{
-				//assert i+d >=N;
-				//assert m != null && d < N == m.Length0 == m.Length1 && i <= N && i+d <= N;
-				//assert SumOnD(m,N,d,i,i+d,s) == SumOnD(m,N,d,i,i+d,s);
-				assert MatrixDiagSum(m,N,d) == SumOnD(m,N,d,i,0,s);
-				if(i-d>=0){
-					assert MatrixDiagSum(m,N,d) == SumOnD(m,N,d,i,0,s);
-					s:=s+m[i,i-d];
-					assert MatrixDiagSum(m,N,d) == SumOnD(m,N,d,i,0,s-m[i,i-d]);
-				}
-				else{
-					assert MatrixDiagSum(m,N,d) == SumOnD(m,N,d,i,0,s);
-				}
-				//in one case we added an element to s and in the other we didn't..
-				//i need to tell dafny that all the other elements in this row definately don't need to be added to the sum s
-				assert MatrixDiagSum(m,N,d) == SumOnD(m,N,d,i,N-1,s);
-
-				assert (MatrixDiagSum(m,N,d) == SumOnD(m,N,d,i,0,s-m[i,i-d])) || (MatrixDiagSum(m,N,d) == SumOnD(m,N,d,i,0,s-m[i,i-d]));
-			}
-
-			assert (MatrixDiagSum(m,N,d) == SumOnD(m,N,d,i,0,s-m[i,i-d])) || (MatrixDiagSum(m,N,d) == SumOnD(m,N,d,i,0,s)) || (MatrixDiagSum(m,N,d) == SumOnD(m,N,d,i,0,s-m[i,i+d])) || (MatrixDiagSum(m,N,d) == SumOnD(m,N,d,i,0,s-m[i,i+d]-m[i,i-d]));
-
-			i:=i+1;
-				assert MatrixDiagSum(m,N,d) == SumOnD(m,N,d,i,0,s);
-		}
-
-		assert i==N;
-		assert MatrixDiagSum(m,N,d) == SumOnD(m,N,d,i,0,s);
-		assert s == MatrixDiagSum(m,N,d);
-
-	}
-
-
-
-/** method MatrixDiagonal(m: array2<int>, N: nat, d: nat) returns (s: int)
-	requires m != null && d < N == m.Length0 == m.Length1
-	ensures s == MatrixDiagSum(m,N,d)
-{
-	/*
-		The following implementation makes N*N checks of "Abs(i-j) == d".
-		Re-implement without any use of "Abs" (make it a simple "function", not a "function method").
-		The challenge is to compute the sum of the relevant elements from each row directly,
-		skipping all irrelevant elements.
-	*/
-	s := 0;
-	var i: nat := 0;
-	while i != N
-		invariant i <= N
-		invariant MatrixDiagSum(m,N,d) == SumOnD(m,N,d,i,0,s)
-		decreases N-i
-	{
-		var j: nat := 0;
-		while j != N
-			invariant j <= N
-			invariant MatrixDiagSum(m,N,d) == SumOnD(m,N,d,i,j,s)
-			decreases N-j
-		{
-			if Abs(i-j) == d
+			calc
 			{
-				s := s+m[i,j];
-			}
-			j := j+1;
+					SumOnD(m,N,d,i,a,s);
+					== 
+					{
+						assert SumOnD(m,N,d,i,a,s)==SumOnD(m,N,d,i,k,s);
+					}
+					SumOnD(m,N,d,i,k,s);
+					== 
+					{
+						assert m != null && d < N == m.Length0 == m.Length1 && i < N && k < N;
+						assert Abs(i-k) != d;
+						L1(m,N,d,i,k,s);
+						assert SumOnD(m,N,d,i,k,s) == SumOnD(m,N,d,i,k+1,s);
+					}
+					SumOnD(m,N,d,i,k+1,s);
+				}	
 		}
-		i := i+1;
+
+		k:=k+1;
+		assert a<=k<=b && SumOnD(m,N,d,i,a,s)==SumOnD(m,N,d,i,k,s);
 	}
+	assert k==b && a<=k<=b && SumOnD(m,N,d,i,a,s)==SumOnD(m,N,d,i,k,s);
+	// ==>
+	assert SumOnD(m,N,d,i,a,s)== SumOnD(m,N,d,i,b,s);
 }
 
-method MatrixDiagonal'(m: array2<int>, N: nat, d: nat) returns (s: int)
-	requires m != null && d < N == m.Length0 == m.Length1
-	ensures s == MatrixDiagSum(m,N,d)
-{
-	s := 0;
-	var i: nat := 0;
-	while i != N
-		invariant i <= N
-		invariant MatrixDiagSum(m,N,d) == SumOnD(m,N,d,i,0,s)
-		decreases N-i
-	{
-		var j: nat := 0;
-		while j != N
-			invariant j <= N
-			invariant MatrixDiagSum(m,N,d) == SumOnD(m,N,d,i,j,s)
-			decreases N-j
-		{
-			assert MatrixDiagSum(m,N,d) == SumOnD(m,N,d,i,j,s);
-			if Abs(i-j) == d
-			{
-				assert m != null && d < N;
-				assert MatrixDiagSum(m,N,d) == SumOnD(m,N,d,i,j,s);
-				assert Abs(i-j) == d;
-				assert i < N && j < N;
-				// ==>
-				assert MatrixDiagSum(m,N,d) == SumOnD(m,N,d,i,j+1,s+m[i,j]);
-				s := s+m[i,j];
-				assert MatrixDiagSum(m,N,d) == SumOnD(m,N,d,i,j+1,s);
-			}
-			else
-			{
-				assert MatrixDiagSum(m,N,d) == SumOnD(m,N,d,i,j,s);
-				assert Abs(i-j) != d;
-				assert i < N && j < N;
-				// ==>
-				assert MatrixDiagSum(m,N,d) == SumOnD(m,N,d,i,j+1,s);
-			}
-			assert MatrixDiagSum(m,N,d) == SumOnD(m,N,d,i,j+1,s);
-			j := j+1;
-		}
-		i := i+1;
-	}
-}*/
-
-
+*/
