ExtremeElements.dfy
@@ -40,6 +40,7 @@ method ExtremeElements(qs: seq<seq<int>>) returns (min: int, max: int)
 	}
 }
 
+
 method EE1(qs: seq<seq<int>>, i0: nat, j0: nat, min0: int, max0: int) returns (i: nat, j: nat, min: int, max: int)
 	requires Inv1(qs,i0,j0,min0,max0)
 	requires i0 != |qs|
@@ -47,7 +48,7 @@ method EE1(qs: seq<seq<int>>, i0: nat, j0: nat, min0: int, max0: int) returns (i
 	ensures 0 <= |qs|-i < |qs|-i0
 	{
 		i,j,min,max:=i0,0,min0,max0;
-		// from postcondition
+
 		assert i0 != |qs|;
 		// from Inv1
 		assert i0 <= |qs|;
@@ -60,25 +61,41 @@ method EE1(qs: seq<seq<int>>, i0: nat, j0: nat, min0: int, max0: int) returns (i
 		
 		assert i < |qs|;
 		
-		if(|qs[i]|>0){
+		if(|qs[i]|>0)
+		{
 			
-			var k1:int :=max1(qs[i]);
-			if(max<k1){
-				max:= k1;
-			}else{}
+			var k1:int :=Max(qs[i]);
+			var k2:int :=Min(qs[i]);
+						
+			if(max<k1) && (min>k2)
+			{
+				max,min:= k1,k2;
+			}
+			else if(max<k1)
+			{
+				max:=k1;
+			}
+			else if(min>k2)
+			{
+				min:=k2;
+			}
+			else
+			{
+			}
 
-			var k2:int :=min1(qs[i]);
-			if(min>k2){
-				min:= k2;
-			}else{}
+		}
+		else
+		{
+		}
 
-		}else{}
 		assert (exists row: nat,column: nat :: ((row < i && column < |qs[row]|) || (row == i < |qs| && column < |qs[i]|)) && min == qs[row][column]);
 		assert (exists row: nat,column: nat :: ((row < i && column < |qs[row]|) || (row == i < |qs| && column < |qs[i]|)) && max == qs[row][column]);
 
 		i:=i+1;
 	
 	}
+
+
 
 predicate Inv1(qs: seq<seq<int>>, i: nat, j: nat, min: int, max: int)
 {
@@ -90,46 +107,243 @@ predicate Inv1(qs: seq<seq<int>>, i: nat, j: nat, min: int, max: int)
 }
 
 
-method max1(a:seq<int>) returns(max:int)
- requires |a|>0;
- ensures (forall j :int :: (j >= 0 && j < |a| ==> max >= a[j]));
- ensures (|a| > 0)==>(exists j : int :: j>=0 && j < |a| && max==a[j]);
+method Max(a:seq<int>) returns(max:int)
+ requires |a|>0
+ ensures (forall j :int :: (j >= 0 && j < |a| ==> max >= a[j]))
+ ensures (|a| > 0)==>(exists j : int :: j>=0 && j < |a| && max==a[j])
 {
-	 if (|a| == 0)  { max := 0;} 
- 
-	 else {
-		 max:=a[0];
-		 var i:int :=1;
-		 while(i < |a|)
-		 invariant (i<=|a|) && (forall j:int :: j>=0 && j<i ==> max >= a[j]) && (exists j:int :: j>=0 && j<i && max==a[j]);
-		 decreases (|a|-i); 
-		 {
-			 if(a[i] > max){max := a[i];}
-			 i := i + 1;
- 
-		 }
-	 }
+
+	max:=a[0];
+	var i:int :=1;
+	while(i < |a|)
+	invariant (i<=|a|) && (forall j:int :: j>=0 && j<i ==> max >= a[j]) && (exists j:int :: j>=0 && j<i && max==a[j])
+	decreases (|a|-i) 
+	{
+		if(a[i] > max)
+		{
+			max := a[i];
+		}
+		i := i + 1;
+	}
+	 
 } 
 
-method min1(a:seq<int>) returns(min:int)
+
+method Min(a:seq<int>) returns(min:int)
  requires |a|>0;
  ensures (forall j :int :: (j >= 0 && j < |a| ==> min <= a[j]));
  ensures (|a| > 0)==>(exists j : int :: j>=0 && j < |a| && min==a[j]);
 {
-	 if (|a| == 0)  { min := 0;} 
- 
-	 else {
-		 min:=a[0];
-		 var i:int :=1;
-		 while(i < |a|)
-		 invariant (i<=|a|) && (forall j:int :: j>=0 && j<i ==> min <= a[j]) && (exists j:int :: j>=0 && j<i && min==a[j]);
-		 decreases (|a|-i); 
-		 {
-			 if(a[i] < min){min := a[i];}
-			 i := i + 1;
- 
-		 }
-	 }
-}
+
+	min:=a[0];
+	var i:int :=1;
+	while(i < |a|)
+	invariant (i<=|a|) && (forall j:int :: j>=0 && j<i ==> min <= a[j]) && (exists j:int :: j>=0 && j<i && min==a[j]);
+	decreases (|a|-i) 
+	{
+		if(a[i] < min)
+		{
+			min := a[i];
+		}
+		i := i + 1;
+	}
+	 
+} 
 
 
+
+/** Annotated Versions */
+
+/**
+
+	method EE1'(qs: seq<seq<int>>, i0: nat, j0: nat, min0: int, max0: int) returns (i: nat, j: nat, min: int, max: int)
+	requires Inv1(qs,i0,j0,min0,max0)
+	requires i0 != |qs|
+	ensures Inv1(qs,i,j,min,max)
+	ensures 0 <= |qs|-i < |qs|-i0
+	{
+
+		i,j,min,max:=i0,0,min0,max0; 
+	
+		assert i0 != |qs|;
+		// from Inv1
+		assert i0 <= |qs|;
+		assert i0 < |qs|; // by i0 != |qs| &&  i0 <= |qs| ==> i0 < |qs|
+		assert i < |qs|; // by i:=i0
+		assert i < |qs| ==> j <= |qs[i]|;
+		assert min <= max;
+		
+		assert (forall row: nat,column: nat :: (row < i && column < |qs[row]|) || (row == i < |qs| && column < j) ==> min <= qs[row][column] <= max);
+		
+		assert i < |qs|;
+		
+		if(|qs[i]|>0)
+		{
+			assert |qs[i]|>0; //if-guard
+			
+			var k1:int :=Max(qs[i]);
+			var k2:int :=Min(qs[i]);
+						
+			if(max<k1) && (min>k2)
+			{
+				assert max<k1 && min>k2; //if-guard
+
+				assert Inv1(qs,i+1,j,k2,k1);
+				assert 0 <= |qs|-(i+1) < |qs|-i0;
+				max,min:= k1,k2;
+				assert Inv1(qs,i+1,j,min,max);
+				assert 0 <= |qs|-(i+1) < |qs|-i0;
+			}
+			else if(max<k1)
+			{
+				assert max<k1; //if-guard
+
+				assert Inv1(qs,i+1,j,min,k1);
+				assert 0 <= |qs|-(i+1) < |qs|-i0;
+				max:=k1;
+				assert Inv1(qs,i+1,j,min,max);
+				assert 0 <= |qs|-(i+1) < |qs|-i0;
+			}
+			else if(min>k2)
+			{
+				assert min>k2; //if-guard
+
+				assert Inv1(qs,i+1,j,k2,max);
+				assert 0 <= |qs|-(i+1) < |qs|-i0;
+				min:=k2;
+				assert Inv1(qs,i+1,j,min,max);
+				assert 0 <= |qs|-(i+1) < |qs|-i0;
+			}
+			else
+			{	
+				assert !(max<k1) && !(min>k2); //not if-guards 
+
+				assert Inv1(qs,i+1,j,min,max);
+				assert 0 <= |qs|-(i+1) < |qs|-i0;
+			}
+			assert Inv1(qs,i+1,j,min,max);
+			assert 0 <= |qs|-(i+1) < |qs|-i0;
+		}
+		else
+		{
+			assert |qs[i]|<=0; //!if-guard
+
+			assert Inv1(qs,i+1,j,min,max);
+			assert 0 <= |qs|-(i+1) < |qs|-i0;
+		}
+
+		assert (exists row: nat,column: nat :: ((row < i && column < |qs[row]|) || (row == i < |qs| && column < |qs[i]|)) && min == qs[row][column]);
+		assert (exists row: nat,column: nat :: ((row < i && column < |qs[row]|) || (row == i < |qs| && column < |qs[i]|)) && max == qs[row][column]);
+
+		assert Inv1(qs,i+1,j,min,max);
+		assert 0 <= |qs|-(i+1) < |qs|-i0;
+
+		i:=i+1;
+		
+		assert Inv1(qs,i,j,min,max);
+		assert 0 <= |qs|-i < |qs|-i0;
+	
+	}
+
+
+method Max'(a:seq<int>) returns(max:int)
+ requires |a|>0;
+ ensures (forall j :int :: (j >= 0 && j < |a| ==> max >= a[j]));
+ ensures (|a| > 0)==>(exists j : int :: j>=0 && j < |a| && max==a[j]);
+{
+	
+	assert |a|>0; //pre-condition
+	
+	max:=a[0];
+
+	assert (1<=|a|) && (forall j:int :: j>=0 && j<1 ==> max >= a[j]) && (exists j:int :: j>=0 && j<1 && max==a[j]);
+
+	var i:int :=1;
+
+	assert (i<=|a|) && (forall j:int :: j>=0 && j<i ==> max >= a[j]) && (exists j:int :: j>=0 && j<i && max==a[j]);
+
+	while(i < |a|)
+	invariant (i<=|a|) && (forall j:int :: j>=0 && j<i ==> max >= a[j]) && (exists j:int :: j>=0 && j<i && max==a[j]);
+	decreases (|a|-i) 
+	{
+		if(a[i] > max)
+		{
+			assert a[i]>max; //guard
+			assert (i+1<=|a|) && (forall j:int :: j>=0 && j<i+1 ==> a[i] >= a[j]) && (exists j:int :: j>=0 && j<i+1 && a[i]==a[j]);
+			max := a[i];
+			assert (i+1<=|a|) && (forall j:int :: j>=0 && j<i+1 ==> max >= a[j]) && (exists j:int :: j>=0 && j<i+1 && max==a[j]);
+		}
+		else
+		{
+			assert a[i]<=max; //!if-guard
+			assert (i+1<=|a|) && (forall j:int :: j>=0 && j<i+1 ==> max >= a[j]) && (exists j:int :: j>=0 && j<i+1 && max==a[j]);
+		}
+		assert (i+1<=|a|) && (forall j:int :: j>=0 && j<i+1 ==> max >= a[j]) && (exists j:int :: j>=0 && j<i+1 && max==a[j]);
+		i := i + 1;
+		assert (i<=|a|) && (forall j:int :: j>=0 && j<i ==> max >= a[j]) && (exists j:int :: j>=0 && j<i && max==a[j]);
+	}
+	assert i>=|a|; //!guard
+	assert (i<=|a|) && (forall j:int :: j>=0 && j<i ==> max >= a[j]) && (exists j:int :: j>=0 && j<i && max==a[j]); //inv
+	
+	//==> 
+	
+	assert i==|a|;
+	assert |a|>0; //pre-cond
+
+	// ==>
+	
+	assert (forall j :int :: (j >= 0 && j < |a| ==> max >= a[j]));
+	assert (|a| > 0)==>(exists j : int :: j>=0 && j < |a| && max==a[j]);
+} 
+
+
+method Min'(a:seq<int>) returns(min:int)
+ requires |a|>0;
+ ensures (forall j :int :: (j >= 0 && j < |a| ==> min <= a[j]));
+ ensures (|a| > 0)==>(exists j : int :: j>=0 && j < |a| && min==a[j]);
+{
+	
+	assert |a|>0; //pre-condition
+
+	min:=a[0];
+	
+	assert (1<=|a|) && (forall j:int :: j>=0 && j<1 ==> min <= a[j]) && (exists j:int :: j>=0 && j<1 && min==a[j]);
+
+	var i:int :=1;
+
+	assert (i<=|a|) && (forall j:int :: j>=0 && j<i ==> min <= a[j]) && (exists j:int :: j>=0 && j<i && min==a[j]);
+
+	while(i < |a|)
+	invariant (i<=|a|) && (forall j:int :: j>=0 && j<i ==> min <= a[j]) && (exists j:int :: j>=0 && j<i && min==a[j]);
+	decreases (|a|-i) 
+	{
+		if(a[i] < min)
+		{
+			assert a[i]<min; //guard
+			assert (i+1<=|a|) && (forall j:int :: j>=0 && j<i+1 ==> a[i] <= a[j]) && (exists j:int :: j>=0 && j<i+1 && a[i]==a[j]);
+			min := a[i];
+			assert (i+1<=|a|) && (forall j:int :: j>=0 && j<i+1 ==> min <= a[j]) && (exists j:int :: j>=0 && j<i+1 && min==a[j]);
+		}
+		else
+		{	
+			assert a[i]>=min; //!if-guard
+			assert (i+1<=|a|) && (forall j:int :: j>=0 && j<i+1 ==> min <= a[j]) && (exists j:int :: j>=0 && j<i+1 && min==a[j]);
+		}
+		assert (i+1<=|a|) && (forall j:int :: j>=0 && j<i+1 ==> min <= a[j]) && (exists j:int :: j>=0 && j<i+1 && min==a[j]);
+		i := i + 1;
+		assert (i<=|a|) && (forall j:int :: j>=0 && j<i ==> min <= a[j]) && (exists j:int :: j>=0 && j<i && min==a[j]);
+	}
+	assert i>=|a|; //!guard
+	assert (i<=|a|) && (forall j:int :: j>=0 && j<i ==> min <= a[j]) && (exists j:int :: j>=0 && j<i && min==a[j]); //inv
+	
+	//==> 
+	
+	assert i==|a|;
+	assert |a|>0; //pre-cond
+	// ==>
+	
+	assert (forall j :int :: (j >= 0 && j < |a| ==> min <= a[j]));
+	assert (|a| > 0)==>(exists j : int :: j>=0 && j < |a| && min==a[j]);
+} 
+
+*/
